working

cpdt/CoalgebraCPDT.v
@@ -1,6 +1,11 @@
 Require Import List.
+Require Import CpdtTactics.
 
 Set Implicit Arguments.
+
+(** Define a [stream] as an infinite structure with a single constructor and
+  no base case.  The [CoInductive] definition is used for this creature, but
+  it looks a great deal like an Inductive type without the base case. *)
 
 Section stream.
   Variable A:Type.
@@ -9,10 +14,22 @@ Section stream.
   | Cons : A -> stream -> stream.
 End stream.
 
+(** [zeros] is a [stream] of [nat]s constructed by consing 0 onto [zeros].
+  This has the feel of an infinite type in Haskell.  Even looks kind of like
+  an infinite type in Haskell. *)
+
 CoFixpoint zeros: stream nat := Cons 0 zeros.
+
+(** Similuar mutual construction of alternating [true] and [false] values. 
+  Note the use of [with] to provide two mutual definitions.  This is the
+  first time I have seen this. *)
 
 CoFixpoint trues_falses: stream bool := Cons true falses_trues
 with falses_trues : stream bool := Cons false trues_falses.
+
+(** [approx] looks at the first [n] elements of stream [s].  Note that
+ [approx] does not evaluate the stream and only looks at the stream head.
+ It uses [n] to define a finite prefix of [s] that is [n] elements long. *)
 
 Fixpoint approx A (s:stream A)(n:nat) : list A :=
   match n with
@@ -26,6 +43,13 @@ Eval simpl in approx zeros 10.
 
 Eval simpl in approx trues_falses 10.
 
+(** Stream [map] is just what you think it would be.  However, stream [map]
+ cannot terminate.  Thus, you can only look at finite prefixes of the stream. 
+ The reference [t], the infinite tail of [s], is *guarded* by the constructor
+ [Cons].  Why does this help?  You can calculate [(f h)] on the head and
+ tuck the tail into a recursive [map] call that *need not be evaluted* to 
+ define the corecursive call.  This guarding is key to the definition. *)
+
 Section map.
   Variables A B : Type.
   Variable f : A -> B.
@@ -36,6 +60,12 @@ Section map.
     end.
 End map.
 
+(** This is not in the book, but shows that the [map] constructs a stream that
+ can be computed with using [approx] or any other similar thing that does not
+ touch the infinite tail. *)
+
+Eval compute in approx (map (fun x => (x + 1)) zeros) 10.
+
 Fixpoint even(n:nat):bool :=
   match n with
   | 0 => true 
@@ -45,6 +75,13 @@ Fixpoint even(n:nat):bool :=
 
 Eval compute in map even zeros.
 
+Eval compute in approx (map even zeros) 10.
+
+(** [interleave] does what the name implies and interleaves to streams.
+  the [CoFixpoint] creates a stream that we can take a peek at later as
+  long as we don't touch the tail.  Note that the call to [interleave] is
+  guarded by the constructor [Cons]. *)
+
 Section interleave.
   Variable A : Type.
   
@@ -53,6 +90,8 @@ Section interleave.
     | Cons h1 t1, Cons h2 t2 => Cons h1 (Cons h2 (interleave t1 t2))
     end.
 End interleave.
+
+Eval compute in approx (interleave zeros zeros) 10.
 
 (** It would seem this function fails because it touches or evaluates a stream.
  One can safely look at some finite part of the stream, but looking at the
@@ -138,3 +177,83 @@ Section stream_eq_coind.
     apply stream_eq_coind.
     apply (Cons_case_tl H).
   Qed.
+End stream_eq_coind.
+
+Print stream_eq_coind.
+
+(** [intuition] and [subst] do quite a bit of work here.  [unfold] makes the
+  [hd] and [tl] visible to the proof.  Thus [reflexivity] can pop things
+  out quickly.  Still, the larger proof is opaque to me. *)
+
+Theorem ones_eq'' : stream_eq ones ones'.
+  apply (stream_eq_coind (fun s1 s2 => s1 = ones /\ s2 = ones')).
+  intuition. subst. unfold ones. unfold ones'. reflexivity.
+  intuition. subst. unfold ones. reflexivity.
+  subst. unfold ones'. reflexivity.
+  intuition.
+Qed.
+
+Section stream_eq_loop.
+  Variable A : Type.
+  Variables s1 s2 : stream A.
+
+  Hypothesis Cons_case_hd: hd s1 = hd s2.
+  Hypothesis loop1 : tl s1 = s1.
+  Hypothesis loop2 : tl s2 = s2.
+
+  Theorem stream_eq_loop: stream_eq s1 s2.
+    apply (stream_eq_coind (fun s1' s2' => s1' = s1 /\ s2' = s2)).
+    intuition. subst s0. subst s3. assumption.
+    intuition. subst s0. assumption.
+    intuition. subst s3. assumption.
+    intuition.
+  Qed.
+End stream_eq_loop.
+
+Theorem ones_eq''' : stream_eq ones ones'.
+  apply stream_eq_loop.
+  intuition. intuition. intuition.
+Qed.
+
+Require Import Arith.
+
+CoFixpoint fact_slow'(n:nat) := Cons (fact n) (fact_slow' (S n)).
+Definition fact_slow := fact_slow' 1.
+
+CoFixpoint fact_iter'(cur acc:nat) := Cons acc (fact_iter' (S cur) (acc*cur)).
+Definition fact_iter := fact_iter' 2 1.
+
+Eval simpl in approx fact_iter 5.
+Eval simpl in approx fact_slow 5.
+
+Lemma fact_def : forall x n,
+    fact_iter' x (fact n * S n) = fact_iter' x (fact (S n)).
+  simpl. intros. f_equal. ring.
+Qed.
+
+Hint Resolve fact_def.
+
+Lemma fact_eq': forall n, stream_eq (fact_iter' (S n) (fact n))(fact_slow' n).
+  intro. apply (stream_eq_coind (fun s1 s2 => exists n, s1 = fact_iter' (S n) (fact n)
+                                                /\ s2 = fact_slow' n)).
+  intros. simpl. crush. crush. eauto. eauto.
+Qed.
+
+Theorem fact_eq'' : stream_eq fact_iter fact_slow.
+  apply fact_eq'.
+Qed.
+
+Section stream_eq_onequant.
+  Variables A B : Type.
+  Variables f g : A -> stream B.
+
+  Hypothesis Cons_case_hd : forall x, hd (f x) = hd (g x).
+  Hypothesis Cons_case_tl : forall x, exists y, tl (f x) = f y /\ tl (g x) = g y.
+
+  Theorem stream_eq_onequant: forall x, stream_eq (f x) (g x).
+    intros; apply (stream_eq_coind (fun s1 s2 => exists x, s1 = f x /\ s2 = g x));
+      crush; eauto.
+  Qed.
+
+  
+  
